NuInstructions.thy
@@ -26,6 +26,7 @@ theorem if_\<nu>proc: "(\<^bold>p\<^bold>r\<^bold>e\<^bold>m\<^bold>i\<^bold>s\<
 
 lemma [simp]: "(if P then (A \<flower> B) else (A' \<flower> B')) = ((if P then A else A') \<flower> (if P then B else B'))" by auto
 lemma [simp]: "(if P then (A\<boxbar>B) else (A'\<boxbar>B')) = ((if P then A else A')\<boxbar>(if P then B else B'))" by auto
+lemma [simp]: "(if P then \<tort_lbrace>T1\<tort_rbrace> else \<tort_lbrace>T2\<tort_rbrace>) = \<tort_lbrace>if P then T1 else T2\<tort_rbrace>"  by auto
 lemma [simp]: "(if P then (x \<tycolon> N) else (y \<tycolon> N)) = ((if P then x else y) \<tycolon> N)"  by auto
 
 
@@ -33,17 +34,65 @@ section \<open>Arithmetic instructions\<close>
 
 \<nu>overloads "+" and round_add and "<" and "-"
 
+
 subsection \<open>Integer arithmetic\<close>
 
-subsubsection \<open>addition\<close>
+subsubsection \<open>constant\<close>
+
+definition op_const_int :: "('w::len) itself \<Rightarrow> ('w::len) word \<Rightarrow> ('r::lrep) \<Rightarrow> ('w word \<times> 'r) state"
+  where "op_const_int _ c r = StatOn (c,r)"
+theorem const_nat_\<nu>proc: "\<^bold>p\<^bold>r\<^bold>o\<^bold>c op_const_int TYPE('w::len) c \<blangle> R \<longmapsto> unat c \<tycolon> \<nat>['w]\<boxbar>R \<brangle>"
+  unfolding \<nu>def op_const_int_def by auto
+
+lemma [\<nu>intro]:
+  "\<^bold>p\<^bold>r\<^bold>e\<^bold>m\<^bold>i\<^bold>s\<^bold>e (numeral x :: nat) < 2^LENGTH('w) \<Longrightarrow>
+   \<^bold>c\<^bold>o\<^bold>n\<^bold>s\<^bold>t\<^bold>r\<^bold>u\<^bold>c\<^bold>t ((numeral x) \<tycolon> \<nat>['w]) \<^bold>b\<^bold>y \<^bold>p\<^bold>r\<^bold>o\<^bold>c op_const_int TYPE('w::len) (Word.of_nat (numeral x)) \<blangle> EoC Z \<longmapsto> (numeral x) \<tycolon> \<nat>['w]\<boxbar>EoC Z \<brangle>"
+  unfolding op_const_int_def \<nu>def including show_more1 apply auto by (metis mod_if unat_bintrunc unat_numeral)
+  \<comment> \<open>Only literal number could be constructed automatically\<close>
+lemma [\<nu>intro]:
+  "\<^bold>c\<^bold>o\<^bold>n\<^bold>s\<^bold>t\<^bold>r\<^bold>u\<^bold>c\<^bold>t (0 \<tycolon> \<nat>['w]) \<^bold>b\<^bold>y \<^bold>p\<^bold>r\<^bold>o\<^bold>c op_const_int TYPE('w::len) 0 \<blangle> EoC Z \<longmapsto> 0 \<tycolon> \<nat>['w]\<boxbar>EoC Z \<brangle>"
+  unfolding EoC_def AutoConstruct_def using const_nat_\<nu>proc by (metis unat_0) 
+lemma [\<nu>intro]:
+  "\<^bold>c\<^bold>o\<^bold>n\<^bold>s\<^bold>t\<^bold>r\<^bold>u\<^bold>c\<^bold>t (1 \<tycolon> \<nat>['w]) \<^bold>b\<^bold>y \<^bold>p\<^bold>r\<^bold>o\<^bold>c op_const_int TYPE('w::len) 1 \<blangle> EoC Z \<longmapsto> 1 \<tycolon> \<nat>['w]\<boxbar>EoC Z \<brangle>"
+  unfolding EoC_def AutoConstruct_def using const_nat_\<nu>proc by (metis unat_1) 
+
+subsubsection \<open>plus\<close>
+
+instantiation typing :: (lrep, plus) plus begin
+definition plus_typing :: "('a,'b) typing \<Rightarrow> ('a,'b) typing \<Rightarrow> ('a,'b) typing"
+  where "nu_of a = nu_of b \<Longrightarrow> plus_typing a b = (case a of xa \<tycolon> Na \<Rightarrow> case b of xb \<tycolon> Nb \<Rightarrow> xa + xb \<tycolon> Na)"
+lemma [simp]: "(x \<tycolon> N) + (y \<tycolon> N) = (x + y \<tycolon> N)" using plus_typing_def by auto
+instance by standard
+end
+
+lemma[\<nu>intro]:
+  "\<^bold>c\<^bold>o\<^bold>n\<^bold>s\<^bold>t\<^bold>r\<^bold>u\<^bold>c\<^bold>t (A,B) \<^bold>b\<^bold>y \<^bold>p\<^bold>r\<^bold>o\<^bold>c f \<blangle> (EoC Z \<flower> W1) \<longmapsto> (xa \<tycolon> Na\<boxbar> xb \<tycolon> Nb\<boxbar>EoC Z \<flower> W2) \<brangle> \<Longrightarrow>
+   \<^bold>c\<^bold>o\<^bold>n\<^bold>s\<^bold>t\<^bold>r\<^bold>u\<^bold>c\<^bold>t (+) \<^bold>b\<^bold>y \<^bold>p\<^bold>r\<^bold>o\<^bold>c add \<blangle> (xa \<tycolon> Na\<boxbar> xb \<tycolon> Nb\<boxbar>EoC Z \<flower> W2) \<longmapsto> (xc \<tycolon> Nc\<boxbar>EoC Z \<flower> W3)\<brangle> \<Longrightarrow>
+   \<^bold>c\<^bold>o\<^bold>n\<^bold>s\<^bold>t\<^bold>r\<^bold>u\<^bold>c\<^bold>t (A + B) \<^bold>b\<^bold>y \<^bold>p\<^bold>r\<^bold>o\<^bold>c (f \<nuInstrComp> add) \<blangle>  (EoC Z \<flower> W1) \<longmapsto> (xc \<tycolon> Nc\<boxbar>EoC Z \<flower> W3) \<brangle>"
+  unfolding EoC_def AutoConstruct_def by rule+
+
 definition op_add :: "nat \<Rightarrow> ('a::len) word \<times> ('a::len) word \<times> ('r::lrep) \<Rightarrow> (('a::len) word \<times> 'r) state"
   where "op_add w p = (case p of (a,b,r) \<Rightarrow> if LENGTH('a) = w then StatOn (a+b, r) else STrap)"
 declare op_add_def[\<nu>instr]
-theorem add_nat[\<nu>overload +]: "\<^bold>p\<^bold>r\<^bold>e\<^bold>m\<^bold>i\<^bold>s\<^bold>e x + y < 2^LENGTH('b) \<Longrightarrow> \<^bold>p\<^bold>r\<^bold>o\<^bold>c op_add (LENGTH('b)) \<blangle> x \<tycolon> \<nat>['b::len] \<boxbar> y \<tycolon> \<nat>['b] \<boxbar> \<RR>emain_stack \<longmapsto> x + y \<tycolon> \<nat>['b] \<boxbar> \<RR>emain_stack \<brangle>"
+
+theorem add_nat_\<nu>proc[\<nu>overload +]:
+  "\<^bold>p\<^bold>r\<^bold>e\<^bold>m\<^bold>i\<^bold>s\<^bold>e x + y < 2^LENGTH('b::len) \<Longrightarrow> \<^bold>p\<^bold>r\<^bold>o\<^bold>c op_add (LENGTH('b)) \<blangle> x \<tycolon> \<nat>['b] \<boxbar> y \<tycolon> \<nat>['b] \<boxbar>\<R> \<longmapsto> x + y \<tycolon> \<nat>['b] \<boxbar>\<R> \<brangle>"
   unfolding op_add_def Procedure_def by (auto simp add: of_nat_inverse) 
+
+lemma[\<nu>intro]:
+  "\<^bold>p\<^bold>r\<^bold>e\<^bold>m\<^bold>i\<^bold>s\<^bold>e x + y < 2^LENGTH('b::len) \<Longrightarrow>
+  \<^bold>c\<^bold>o\<^bold>n\<^bold>s\<^bold>t\<^bold>r\<^bold>u\<^bold>c\<^bold>t (+) \<^bold>b\<^bold>y \<^bold>p\<^bold>r\<^bold>o\<^bold>c op_add (LENGTH('b)) \<blangle> x \<tycolon> \<nat>['b] \<boxbar> y \<tycolon> \<nat>['b] \<boxbar>EoC Z \<longmapsto> x + y \<tycolon> \<nat>['b] \<boxbar>EoC Z \<brangle>"
+  unfolding AutoConstruct_def EoC_def by (auto simp add: add_nat_\<nu>proc)
+lemma[\<nu>intro]:
+  "\<^bold>p\<^bold>r\<^bold>e\<^bold>m\<^bold>i\<^bold>s\<^bold>e x + y < 2^LENGTH('b::len) \<Longrightarrow> \<^bold>p\<^bold>r\<^bold>o\<^bold>c f \<blangle> EoC Z \<longmapsto> x \<tycolon> \<nat>['b] \<boxbar> y \<tycolon> \<nat>['b] \<boxbar>EoC Z \<brangle> \<Longrightarrow>
+  \<^bold>p\<^bold>r\<^bold>o\<^bold>c (f \<nuInstrComp> op_add (LENGTH('b))) \<blangle> EoC Z \<longmapsto> \<tort_lbrace>(x \<tycolon> \<nat>['b]) + (y \<tycolon> \<nat>['b])\<tort_rbrace> \<boxbar>EoC Z \<brangle>"
+  by (auto simp add: add_nat_\<nu>proc)
+
 
 theorem add_nat_mod[\<nu>overload round_add]: "\<^bold>p\<^bold>r\<^bold>o\<^bold>c op_add (LENGTH('b)) \<blangle> x \<tycolon> \<nat>['b::len] \<boxbar> y \<tycolon> \<nat>['b] \<boxbar> \<RR> \<longmapsto> ((x + y) mod 2^(LENGTH('b))) \<tycolon> \<nat>['b] \<boxbar> \<RR> \<brangle>"
   unfolding op_add_def Procedure_def by (auto simp add: unat_word_ariths)
+
+
 
 subsubsection \<open>subtraction\<close>
 definition op_sub :: "('a::len) itself \<Rightarrow> 'a word \<times> 'a word \<times> ('r::lrep) \<Rightarrow> ('a word \<times> 'r) state"
@@ -60,6 +109,17 @@ theorem op_lt_\<nu>proc[\<nu>overload <]: "\<^bold>p\<^bold>r\<^bold>o\<^bold>c 
   unfolding \<nu>def op_lt_def by (auto simp add: word_less_nat_alt)
 
 section \<open>Tests\<close>
+
+ML \<open>Locale.get_locales @{theory}\<close>
+ML \<open>val ctx = Locale.init "NuPrim.ceq_lrep" @{theory}
+val x = Assumption.all_prems_of ctx\<close>
+
+schematic_goal [simplified, simplified \<nu>post_construct]:
+  "\<^bold>c\<^bold>o\<^bold>n\<^bold>s\<^bold>t\<^bold>r\<^bold>u\<^bold>c\<^bold>t (233 \<tycolon> \<nat>[32], ((copy_reg::((32 word register \<times> 32 word register), (32 word register \<times> 32 word register), (32 word) register, 32 word register) address \<Rightarrow> (32 word, nat) typing)) (address_left address_here)
++ (233 \<tycolon>  \<nat>[32])) \<^bold>b\<^bold>y \<^bold>p\<^bold>r\<^bold>o\<^bold>c ?f \<blangle>((?Z1::(?'a::lrep) set) \<flower> \<^bold>r\<^bold>e\<^bold>g\<^bold>i\<^bold>s\<^bold>t\<^bold>e\<^bold>r A = \<tort_lbrace> 16 \<tycolon> \<nat>[32]\<tort_rbrace> and_ty \<^bold>r\<^bold>e\<^bold>g\<^bold>i\<^bold>s\<^bold>t\<^bold>e\<^bold>r B = \<tort_lbrace> 0 \<tycolon> \<nat>[32] \<tort_rbrace>) \<longmapsto> (?Z2::(?'b::lrep) set) \<brangle>"
+  by  (\<nu>resolve \<nu>intro (\<nu>intro')) 
+
+ thm \<nu>intro
 
 definition [simp]:"difference x y = (if x < y then y - x else x - y)"
 
